\documentclass{article}
\usepackage[utf8]{inputenc}
\usepackage[english]{babel}
\usepackage{listings}
\usepackage{graphicx}

\usepackage[comma,square,numbers,sort&compress]{natbib}
\usepackage{hyperref}

\begin{document}

\begin{flushright}
\bf{Mohammad Saleh\\
GRA at PHY WSU\\
m.saleh@cern.ch\\ fa9520@wayne.edu\\
Feb 15, 2017}
\end{flushright}

\begin{center}
\bf{CSC 5825 \\
Homework 2 } \\
\end{center}
Please don't remove points because I am submitting the homework late. We did exchanged emails that I had a conference for 8 days and got approval for extending the submission date without penalty.
\section*{Solutions:}
\bf{Question 1:}
\newline
$P(x_{1},x_{2},...)=\prod_{i} p_{i}^{x_{i}}$
\newline
log likelihood $L(\bf{p}|x)=\log\prod_{i=1}^{N}\prod_{i=1}^{K}p_{i}^{x_{i}^{t}}=\sum_{t=1}^{N}\sum_{i=1}^{K}\log p_{i}^{x_{i}^{t}}$
\newline
$\frac{\partial L(\bf{r}|x)}{\partial p_{i}}=\frac{\partial[\sum_{t=1}^{N}\sum_{i=1}^{K}x_{i}^{t}.\log p_{i}+\lambda(\sum_{i=1}^{K}p_{i}-1)]}{\partial p_{i}}=0$ ; where $\lambda$ is lagrange multiplier
\newline
$\Rightarrow \sum_{t=1}^{N}x_{i}^{t}.\frac{1}{p_{i}}+\lambda=0$ \newline
$\Rightarrow$$p_{i}=-\frac{1}{\lambda}\sum_{t=1}^{N}x_{i}^{t}$  \newline
$\Rightarrow\sum_{i=1}^{K}x_{i}=1=-\frac{1}{\lambda}\sum_{t=1}^{N}(\sum_{i=1}^{K}x_{i}^{t})$ ; where $\sum_{i=1}^{K}x_{i}^{t}=1$
\newline
$\Rightarrow$ $\lambda=-N$ \newline
$\Rightarrow$ $\hat{p}_{i}=\frac{\sum_{t=1}^{N}x_{i}^{t}}{N}$
\\\\
\bf{Question 2:}
\newline
$\log\frac{P(C_{1}|x)}{P(C_{2}|x)}=\log(P(x|C_{1}))+\log(P(C_{1}))-\log(P(x|C_{2}))-\log(P(C_{2}))$;   according to equation 5.16 page 100 \newline

$\log\frac{P(C_{1}|x)}{P(C_{2}|x)}=(-1/2)\log(|\bf{S_{1}}|)+(1/2)\log(|\bf{S_{2}}|)-
(1/2)(\bf{x}-\bf{\mu_{1}})^{T}\bf{S}_{1}^{-1}(\bf{x}-\bf{\mu_{1}})+
(1/2) (\bf{x}-\bf{\mu_{2}})^{T}\bf{S}_{2}^{-1} (\bf{x}-\bf{\mu_{2}})+\log(P(C_{1}))-\log(P(C_{2}))$
\newline
\newline
--We will start with the simpler case: \\ \\
1-for Hyperspheric case:
$\bf{S_{i}}=\bf{S}=s^{2}\bf{I};~~\bf{S_{1}} =\bf{S_{2}}=s^{2}\bf{I}$ \hfill \break
$\Rightarrow\log\frac{P(C_{1}|x)}{P(C_{2}|x)}=-
(1/2)\bf{s}^{2}(\bf{x}-\bf{\mu_{1}})^{T}(\bf{x}-\bf{\mu_{1}})+
(1/2)\bf{s}^{2}(\bf{x}-\bf{\mu_{2}})^{T}(\bf{x}-\bf{\mu_{2}})+\log(P(C_{1}))-\log(P(C_{2}))$  \newline
\\
2-for Axis-aligned:
\newline
$\bf{S_{i}}=\bf{S}$ with $s_{ij}=0$ , we have $\bf{S_{1}}=\bf{S_{2}}=\bf{S}$
$\Rightarrow$ $\log\frac{P(C_{1}|x)}{P(C_{2}|x)}=-
(1/2)(\bf{x}-\bf{\mu_{1}})^{T}\bf{S}^{-1}(\bf{x}-\bf{\mu_{1}})+
(1/2) (\bf{x}-\bf{\mu_{2}})^{T}\bf{S}^{-1} (\bf{x}-\bf{\mu_{2}})+\log(P(C_{1}))-\log(P(C_{2}))$   \newline
\\
3-for Shared Hyperellipsoidal case:
$\bf{S_{i}}=\bf{S}$ we still have $\bf{S_{1}}=\bf{S_{2}}=\bf{S}$
$\Rightarrow$ $\log\frac{P(C_{1}|x)}{P(C_{2}|x)}=-
(1/2)(\bf{x}-\bf{\mu_{1}})^{T}\bf{S}^{-1}(\bf{x}-\bf{\mu_{1}})+
(1/2) (\bf{x}-\bf{\mu_{2}})^{T}\bf{S}^{-1} (\bf{x}-\bf{\mu_{2}})+\log(P(C_{1}))-\log(P(C_{2}))$   \newline
\\
4-for Different Hyperellipsoidal case:
 we have $\bf{S_{1}}\neq\bf{S_{2}}=\bf{S}$, we end up with the general case
 \\ \\
 $\log\frac{P(C_{1}|x)}{P(C_{2}|x)}=(-1/2)\log(|\bf{S_{1}}|)+(1/2)\log(|\bf{S_{2}}|)-
 (1/2)(\bf{x}-\bf{\mu_{1}})^{T}\bf{S}_{1}^{-1}(\bf{x}-\bf{\mu_{1}})+
 (1/2) (\bf{x}-\bf{\mu_{2}})^{T}\bf{S}_{2}^{-1} (\bf{x}-\bf{\mu_{2}})+\log(P(C_{1}))-\log(P(C_{2}))$
 \newline
\\
\\
\\
\\
\\
\\
\\
\bf{Question 3:}
\newline
Below is the syntax for all the parts of the homework. I did add comments in order to make it more clear. I did also include a snapshot for the compiled code. I used numpy library for dealing with arrays only for simpler syntax(multiplying, mean, ... etc) but didn't use any main
libraries for the question
\begin{figure}
  \includegraphics[scale=0.3]{code_2}
  \caption{snapshot of my code after compiling. It shows all the requested output (MSE) for the homework.}
\end{figure}

\lstinputlisting[language=Python]{HomeWork_2.py}

\end{document}
